

Macroeconomic Theory

Francesco Franco

T3 2026

The Supply Side

New Keynesian Phillips Curve

Remember we have derived the NKPC in terms of marginal cost:

$$\pi_t = \beta E_t \{ \pi_{t+1} \} + \lambda (mc_t + \mu)$$

where $\lambda \equiv \frac{(1-\theta)(1-\beta\theta)}{\theta} \Theta$, $\Theta = \frac{1-\alpha}{1-\alpha+\alpha\epsilon}$

The marginal cost is:

$$mc_t = (w_t - p_t) - (z_t - \alpha n_t + \log(1 - \alpha))$$

The Supply Side

Using labor supply and technology

We used the labor supply condition:

$$w_t - p_t = \sigma c_t + \varphi n_t$$

Combined with technology $n_t = \frac{1}{1-\alpha}(y_t - z_t)$ and goods market equilibrium to obtain:

$$mc_t = \left(\sigma + \frac{\varphi + \alpha}{1 - \alpha} \right) y_t - \left(1 + \frac{\varphi + \alpha}{1 - \alpha} \right) z_t - \log(1 - \alpha)$$

The Supply Side

Flexible prices and output gap

In the flexible prices equilibrium, real marginal cost is constant and equal to $-\mu$:

$$mc = \left(\sigma + \frac{\varphi + \alpha}{1 - \alpha} \right) y_t^n - \left(1 + \frac{\varphi + \alpha}{1 - \alpha} \right) z_t - \log(1 - \alpha)$$

where y_t^n is the natural level of output.

Combining with the NKPC, we get the dynamic IS curve:

$$\tilde{y}_t = E_t\{\tilde{y}_{t+1}\} - \frac{1}{\sigma}(i_t - E_t\{\pi_{t+1}\} - r_t^n)$$

where \tilde{y}_t is the output gap

Notes on the NKM Solution

The three-equation system

Consider the NKM model with:

Monetary Policy Rule:

$$i_t = \rho + \phi_\pi \pi_t + v_t$$

Dynamic IS Curve:

$$\tilde{y}_t = E_t\{\tilde{y}_{t+1}\} - \frac{1}{\sigma}(i_t - E_t\{\pi_{t+1}\} - r_t^n)$$

New Keynesian Phillips Curve:

Notes on the NKM Solution

Key definitions

- ▷ \tilde{y}_t is the **output gap**
- ▷ r_t^n is the **natural rate** of real interest rate — the rate that implies zero output gap
- ▷ $r_t^n = \rho - \sigma(1 - \rho_z)\psi_{yz}z_t$

Household First Order Conditions

Classical model conditions

The first order conditions with respect to C_t and A_t are:

Labor Supply:

$$w_t - p_t = \sigma c_t + \varphi n_t$$

Euler Equation:

$$c_t = E_t\{c_{t+1}\} - \frac{1}{\sigma}(i_t - E_t\{\pi_{t+1}\} - \rho)$$

Notes on the NKM Solution

System reduction

Three endogenous variables: i_t , π_t , \tilde{y}_t

Two exogenous variables: z_t , v_t

Substitute the monetary policy rule into the IS curve:

$$\tilde{y}_t = E_t\{\tilde{y}_{t+1}\} - \frac{1}{\sigma}(\rho + \phi_\pi \pi_t + v_t - E_t\{\pi_{t+1}\} - r_t^n)$$

Combined with the New Keynesian Phillips Curve:

$$\pi_t = \beta E_t\{\pi_{t+1}\} + \kappa \tilde{y}_t$$

Notes on the NKM Solution

Solution guess

Assume a unique solution where endogenous variables respond to state variables:

$$\tilde{y}_t = \psi_{yu} u_t$$

$$\pi_t = \psi_{\pi u} u_t$$

where $u_t = v_t - (r_t^n - \rho)$ is the difference between the two shocks.

We need to determine the unknown coefficients ψ_{yu} , $\psi_{\pi u}$ through guess and verify.

Notes on the NKM Solution

Simplified case: monetary shock only

For simplicity, consider $z_t = 0$ (no technology shock), so $r_t^n = \rho$ and $u_t = v_t$

Assume $v_t \sim N(0, 1)$ is i.i.d. Plugging our guess into the model:

$$\tilde{y}_t = E_t\{\tilde{y}_{t+1}\} - \frac{1}{\sigma}(\phi_\pi \pi_t + u_t - E_t\{\pi_{t+1}\})$$

This becomes:

$$\tilde{y}_t = -\frac{1}{\sigma}(\phi_\pi \psi_{\pi u} + 1)u_t$$

Notes on the NKM Solution

Using the NKPC

Using our guess in the NKPC:

$$\pi_t = \beta E_t\{\pi_{t+1}\} + \kappa \tilde{y}_t$$

Substituting the guess:

$$\pi_t = \beta E_t\{\psi_{\pi u} u_{t+1}\} + \kappa \psi_{yu} u_t$$

Since $E_t u_{t+1} = 0$:

$$\pi_t = \kappa \psi_{yu} u_t$$

Notes on the NKM Solution

Solving for coefficients

To be consistent with our guess, we need:

$$\psi_{yu} = -\frac{1}{\sigma}(\phi_{\pi}\psi_{\pi u} + 1)$$

$$\psi_{\pi u} = \kappa\psi_{yu}$$

Solving these two equations yields:

$$\psi_{yu} = -\frac{1}{\sigma + \phi_{\pi}\kappa}$$

Notes on the NKM Solution

Uniqueness condition

To ensure unique solution, check eigenvalues of matrix A_T are less than unity:

$$\begin{bmatrix} \tilde{y}_t \\ \pi_t \end{bmatrix} = A_T \begin{bmatrix} E_t\{\tilde{y}_{t+1}\} \\ E_t\{\pi_{t+1}\} \end{bmatrix} + B_T u_t$$

where $u_t \equiv \hat{r}_t^n - v_t$ and

$$A_T \equiv \Omega \begin{bmatrix} \sigma & 1 - \beta\phi_\pi \\ \sigma\kappa & \kappa + \beta\sigma \end{bmatrix}; B_T \equiv \Omega \begin{bmatrix} 1 \\ \kappa \end{bmatrix}$$

Notes on the NKM Solution

Jump variables intuition

The dynamics require both variables to have free initial values:

- ▶ After a shock, both output gap and inflation can take correct values ensuring unique solution
- ▶ Both variables are **jump variables** (like consumption in Ramsey model)
- ▶ Unlike capital in Ramsey (state variable), these have no predetermined values
- ▶ State variables require eigenvalue larger than unity in the system formulation

General Solution

Ensuring unique solution

How to solve and ensure unique solution (saddle property)?

Rewrite the system:

$$\begin{bmatrix} E_t\{\tilde{y}_{t+1}\} \\ E_t\{\pi_{t+1}\} \end{bmatrix} = A_D \begin{bmatrix} \tilde{y}_t \\ \pi_t \end{bmatrix} + B_D u_t$$

Decouple dynamics using decomposition:

$$A_D = C \Lambda C^{-1}$$

General Solution

System transformation

The system becomes:

$$\begin{bmatrix} E_t\{\tilde{y}_{t+1}\} \\ E_t\{\pi_{t+1}\} \end{bmatrix} = C\Lambda C^{-1} \begin{bmatrix} \tilde{y}_t \\ \pi_t \end{bmatrix} + B_D u_t$$

Premultiply by C^{-1} :

$$C^{-1} \begin{bmatrix} E_t\{\tilde{y}_{t+1}\} \\ E_t\{\pi_{t+1}\} \end{bmatrix} = \Lambda C^{-1} \begin{bmatrix} \tilde{y}_t \\ \pi_t \end{bmatrix} + C^{-1} B_D u_t$$

$$\text{Define } \tilde{v}_t = C^{-1} \begin{bmatrix} \tilde{y}_t \\ \pi_t \end{bmatrix} \text{ and } \tilde{u}_t = C^{-1} B_D u_t$$

General Solution

Forward iteration

Rearranging: $X_t = \Lambda^{-1} E_t X_{t+1} - \Lambda^{-1} D u_t$

Using Law of Iterated Expectations $E_t E_{t+1} = E_t$:

$$X_t = \sum_{i=1}^{\infty} (\Lambda^{-1})^i E_t [X_{t+i} - D u_{t+i}] - \Lambda^{-1} D u_t$$

Since $E_t [D u_{t+i}] = 0$ for $i > 0$ and both eigenvalues greater than 1:

$$X_t = -\Lambda^{-1} D u_t$$

Transforming back to original system:

Optimal Price Condition

Basic formulation

The optimal price condition gives:

$$p_t^* = (1 - \beta\theta) \sum_{k=0}^{\infty} (\beta\theta)^k E_t \left((\psi_{t+k} + \mu) - \frac{\alpha\epsilon}{1-\alpha} (p_t^* - p_{t+k}) \right)$$

which can be rewritten as:

$$p_t^* = (1 - \beta\theta) \sum_{k=0}^{\infty} (\beta\theta)^k E_t (\Theta (\psi_{t+k} - p_{t+k} + \mu) + p_{t+k})$$

where $\Theta = \frac{1-\alpha}{1-\alpha+\alpha\epsilon}$

Optimal Price Condition

Recursive form

The recursive form is:

$$p_t^* = (1 - \beta\theta) (\Theta (\psi_t - p_t + \mu) + p_t) + \beta\theta E_t p_{t+1}^*$$

Subtracting p_{t-1} :

$$p_t^* - p_{t-1} = (1 - \beta\theta) (\Theta (\psi_t - p_t + \mu) + p_t) - p_{t-1} + \beta\theta E_t p_{t+1}^*$$

Using $\pi_t = p_t - p_{t-1} = (1 - \theta) (p_t^* - p_{t-1})$ to get the NKPC:

$$\pi_t = \lambda (\psi_t - p_t + \mu) + \beta E_t \{\pi_{t+1}\}$$

NK-Phillips Curve

Final form

Replacing in the NKPC:

$$\pi_t = \beta E_t\{\pi_{t+1}\} + \lambda (mc_t + \mu)$$

where:

- ▷ $mc_t = \psi_t - p_t$ is the marginal cost
- ▷ $\lambda \equiv \frac{(1-\theta)(1-\beta\theta)}{\theta} \Theta$
- ▷ $\Theta = \frac{1-\alpha}{1-\alpha+\alpha\epsilon}$

(Solve forward to get the forward-looking structure)

Equilibrium

Goods market clearing

Clearing in the continuum of goods markets:

$$Y_t(i) = C_t(i)$$

Aggregating:

$$Y_t \equiv \left(\int_0^1 Y_t(i)^{1-\frac{1}{\epsilon}} di \right)^{\frac{\epsilon}{\epsilon-1}} = C_t$$

In log-linear form:

Labor Market Clearing

Aggregation across firms

Labor market clearing:

$$N_t = \int_0^1 N_t(i) di$$

Using firm labor demand:

$$N_t = \int_0^1 \left(\frac{Y_t(i)}{Z_t} \right)^{\frac{1}{1-\alpha}} di$$

This gives:

Labor Market Clearing

Labor supply and marginal cost

The labor supply is:

$$w_t - p_t = \sigma c_t + \varphi n_t$$

Using labor demand and technology:

$$mc_t = (w_t - p_t) - (z_t - \alpha n_t + \log(1 - \alpha))$$

Substituting:

$$mc_t = (\sigma y_t + \varphi n_t) - (z_t - \alpha n_t + \log(1 - \alpha))$$

Natural Level of Output and Markup Gap

Flexible prices benchmark

The natural level of output prevails with flexible prices (constant markup):

$$mc = \left(\sigma + \frac{\varphi + \alpha}{1 - \alpha} \right) y_t^n - \left(1 + \frac{\varphi + \alpha}{1 - \alpha} \right) z_t - \log(1 - \alpha)$$

The marginal cost gap is therefore:

$$(mc_{t|t} - mc) = \left(\sigma + \frac{\varphi + \alpha}{1 - \alpha} \right) (y_t - y_t^n)$$

The New Keynesian Phillips Curve

Final specification

Substituting the marginal cost gap gives the NKPC:

$$\pi_t = \beta E_t\{\pi_{t+1}\} + \lambda \left(\sigma + \frac{\varphi + \alpha}{1 - \alpha} \right) (y_t - y_t^n)$$

More compactly:

$$\pi_t = \beta E_t\{\pi_{t+1}\} + \kappa \tilde{y}_t$$

This is the first equation of our NK model.

The C-S Condition (Dynamic IS)

From Euler equation to output gap

The Euler condition plus goods market equilibrium gives:

$$y_t = E_t\{y_{t+1}\} - \frac{1}{\sigma}(i_t - E_t\{\pi_{t+1}\} - \rho)$$

Rewritten in terms of output gap:

$$\tilde{y}_t = E_t\{\tilde{y}_{t+1}\} - \frac{1}{\sigma}(i_t - E_t\{\pi_{t+1}\} - r_t^n)$$

where $r_t^n = \rho - \sigma(1 - \rho_z)\psi_{yz}z_t$ is the **natural rate of interest** (Wicksellian)

The C-S Condition (Dynamic IS)

Definition of natural rate

Definition of r_t^n :

$$y_t^n = E_t [y_{t+1}^n] - \frac{1}{\sigma} (r_t^n - \rho)$$

Therefore:

$$r_t^n = \rho + \sigma E_t [y_{t+1}^n - y_t^n]$$

Using the solution $y_t^n = \psi_y + \psi_{yz} z_t$ and $z_t = \rho_z z_{t-1} + \epsilon_t^z$

Express the Dynamic IS in terms of $\tilde{y} = y - y^n$

The Policy Block

Completing the model

To determine the nominal side of the economy, we need an equation for the nominal interest rate.

We need a rule that gives **determinacy** of equilibrium.

Without a monetary policy rule, the nominal variables would be indeterminate in this model.

Interest Rate Rule

Simple Taylor rule

Consider the following rule:

$$i_t = \rho + \phi_\pi \pi_t + v_t$$

where v_t is a monetary policy shock.

The complete model is now:

$$\tilde{y}_t = E_t\{\tilde{y}_{t+1}\} - \frac{1}{\sigma}(i_t - E_t\{\pi_{t+1}\} - r_t^n)$$

$$\pi_t = \beta E_t\{\pi_{t+1}\} + \kappa \tilde{y}_t$$

Dynamics

Matrix representation

The system is:

$$\begin{bmatrix} \tilde{y}_t \\ \pi_t \end{bmatrix} = A_T \begin{bmatrix} E_t\{\tilde{y}_{t+1}\} \\ E_t\{\pi_{t+1}\} \end{bmatrix} + B_T u_t$$

where $u_t \equiv \hat{r}_t^n - v_t$ and:

$$A_T \equiv \Omega \begin{bmatrix} \sigma & 1 - \beta\phi_\pi \\ \sigma\kappa & \kappa + \beta\sigma \end{bmatrix}; B_T \equiv \Omega \begin{bmatrix} 1 \\ \kappa \end{bmatrix}$$